theories/case_studies/stack_object/stack_object_adequacy.v
@@ -90,7 +90,6 @@ Definition is_initial_memory `{@memory_layout MP} (mem: Mem) :=
   (* instantiating main *)
   ∧ (cmpt_imports main_cmpt) =
   so_main_imports
-    b_switcher e_switcher a_switcher_call ot_switcher
     (b_assert assert_cmpt) (e_assert assert_cmpt) C_f
   ∧ (cmpt_code main_cmpt) = so_main_code
   ∧ (cmpt_data main_cmpt) = so_main_data
