theories/switcher/switcher_spec_return.v
@@ -18,7 +18,7 @@ Section Switcher.
     {stsg : STSG Addr region_type Σ} {cstackg : CSTACKG Σ} {heapg : heapGS Σ}
     {nainv: logrel_na_invs Σ}
     `{MP: MachineParameters}
-    {swlayout : switcherLayout}
+    {swlayout : switcherLayout} {swlayoutwf : switcherLayoutWf}
   .
 
   Implicit Types W : WORLD.
